tmp

Snlean/Lambda.lean
@@ -13,40 +13,49 @@ inductive Term
 | lam : String → Ty → Term → Term
 | app : Term → Term → Term
 deriving BEq, DecidableEq, Repr
-open Term
-prefix:90 "` " => var
-notation:50 "λ " x " : " T " ⬝ " d => lam x T d
-infixr:min " $ " => app
 
+namespace Term
+  prefix:90 "` " => var
+  notation:50 "λ " x " : " T " ⬝ " d => lam x T d
+  infixr:min " $ " => app
+
+  inductive Value : Term → Prop
+  | lam : Value (λ x : T ⬝ e)
+
+  def subst : Term → String → Term → Term
+  | ` x, y, v => if x = y then v else ` x
+  | λ x : T ⬝ b, y, v => if x = y then λ x : T ⬝ b else λ x : T ⬝ (subst b y v)
+  | app l m, y, v => app (subst l y v) (subst m y v)
+  notation:90 " [ " x " := " v " ] " t => subst t x v
+
+  inductive Reduction : Term → Term → Prop
+  | eAppAbs : Value v → Reduction ((λ x : T ⬝ e) $ v) ([x := v] e)
+  | eAppLeft : Reduction e1 e1' → Reduction (e1 $ e2) (e1' $ e2)
+  | eAppRight : Value v → Reduction e2 e2' → Reduction (v $ e2) (v $ e2')
+  open Reduction
+  infix:40 " —→ " => Reduction
+end Term
 
 def TyCtx := List (String × Ty) deriving BEq, DecidableEq, Repr
-def nil : TyCtx := []
-def extend : TyCtx → String → Ty → TyCtx := fun Γ x t => (x, t) :: Γ
-notation "∅" => nil
-def elem : TyCtx → (String × Ty) → Prop
-| []         , _ => false
-| (y, s) :: Γ, (x, t) => if x = y then t = s else elem Γ (x, t)
-infix:50 " ∋ " => elem
+namespace TyCtx
+  open Term
 
-inductive HasType : TyCtx → Term → Ty → Prop
-| tyVar : (Γ ∋ (x, t)) → HasType Γ (var x) t
-| tyAbs : HasType ((x, t1) :: Γ) e t2 → HasType Γ (λ x : t1 ⬝ e) (t1 :→ t2)
-| tyApp : HasType Γ e1 (t2 :→ t1) → HasType Γ e2 t2 → HasType Γ (e1 $ e2) t1
-open HasType
-notation:40 Γ " ⊢ " t " : " ty:51 => HasType Γ t ty
+  def nil : TyCtx := []
+  def extend : TyCtx → String → Ty → TyCtx := fun Γ x t => (x, t) :: Γ
 
-inductive Value : Term → Prop
-| lam : Value (λ x : T ⬝ e)
+  -- `‚` is not a comma! See: <https://www.compart.com/en/unicode/U+201A>
+  notation:50 c " ‚  " s:51 " : " t:51 => extend c s t
 
-def subst : Term → String → Term → Term
-| ` x, y, v => if x = y then v else ` x
-| λ x : T ⬝ b, y, v => if x = y then λ x : T ⬝ b else λ x : T ⬝ (subst b y v)
-| app l m, y, v => app (subst l y v) (subst m y v)
-notation:90 " [ " x " := " v " ] " t => subst t x v
+  -- notation "∅" => nil
+  def elem : TyCtx → (String × Ty) → Prop
+  | []         , _ => false
+  | (y, s) :: Γ, (x, t) => if x = y then t = s else elem Γ (x, t)
+  infix:50 " ∋ " => elem
 
-inductive Reduction : Term → Term → Prop
-| eAppAbs : Value v → Reduction ((λ x : T ⬝ e) $ v) ([x := v] t)
-| eAppLeft : Reduction e1 e1' → Reduction (e1 $ e2) (e1' $ e2)
-| eAppRight : Value v → Reduction e2 e2' → Reduction (v $ e2) (v $ e2')
-open Reduction
-infix:40 " —→ " => Reduction
+  inductive HasType : TyCtx → Term → Ty → Prop
+  | tyVar : (Γ ∋ (x, t)) → HasType Γ (` x) t
+  | tyAbs : HasType ((x, t1) :: Γ) e t2 → HasType Γ (λ x : t1 ⬝ e) (t1 :→ t2)
+  | tyApp : HasType Γ e1 (t2 :→ t1) → HasType Γ e2 t2 → HasType Γ (e1 $ e2) t1
+  open HasType
+  notation:40 Γ " ⊢ " t " : " ty:51 => HasType Γ t ty
+end TyCtx
