Snlean/Soundness.lean
@@ -1,25 +1,32 @@
 import Snlean.Lambda
 
+open Lambda
+
 namespace Soundness
 
-open Lambda
-open Lambda.Reduction
+open TyCtx TyCtx.HasType
+open Term Term.Reduction
 
 -- Issues
 -- progressの停止性
 -- preservationのihe1, ihe2の形式
 
 theorem progress :
-  ∅ ⊢ t : T → Value t ∨ (∃t' : Term, t —→ t')
+  Γ ⊢ t : T ∧ (Γ = nil) → Value t ∨ (∃t' : Term, t —→ t')
 := by
-  intro jt;
-  cases jt with
+  intro assum;
+  have jt := And.left assum;
+  have env_is_emp := And.right assum;
+  induction jt with
   -- Contradictory because env_is_emp contradicts x_elem_env
-  | tyVar _ => contradiction
+  | tyVar x_elem_env =>
+    rw [env_is_emp] at x_elem_env
+    contradiction
   -- Straightforward because t is value
   | tyAbs _ => exact Or.inl Value.lam
-  | @tyApp _ _ _ _ e2 jt1 jt2 =>
-    cases progress jt1 with
+  | tyApp jt1 jt2 ihe1 ihe2 =>
+    have pre_ihe1 := And.intro jt1 env_is_emp;
+    cases ihe1 pre_ihe1 env_is_emp with
     | inr t1_canbe_reduced =>
       cases t1_canbe_reduced with
       | intro t1' t1_canbe_reduced' =>
@@ -30,15 +37,16 @@ theorem progress :
     | inl t1_is_value =>
       apply Or.intro_right
       cases t1_is_value with
-        | @lam x _ e =>
-          cases progress jt2 with
+        | lam =>
+          have pre_ihe2 := And.intro jt2 env_is_emp;
+          cases ihe2 pre_ihe2 env_is_emp with
           -- (λ x1 : T1. t1) $ v —→ [x1 := v] t1
           | inl t2_is_value =>
-              -- apply (Exists.intro _ (eAppAbs t2_is_value))
+            cases t2_is_value with
+            | lam =>
               apply Exists.intro
               apply eAppAbs
-              apply (subst e x e2) -- なんでもOK
-              apply t2_is_value
+              apply Value.lam
           | inr t2_canbe_reduced =>
             cases t2_canbe_reduced with
             | intro _ t2_canbe_reduced' =>
@@ -47,34 +55,74 @@ theorem progress :
               apply Value.lam
               apply t2_canbe_reduced'
 
+
 theorem subst_preservation :
   Γ ⊢ s : S →
-  (x, S) :: Γ ⊢ t : T →
+  Γ' ⊢ t : T ∧ (Γ' = (Γ ‚ x : S)) →
   Γ ⊢ [x := s] t : T
 := by
+  intro js assum_t;
+  have jt := And.left assum_t;
+  have x_elem_gamma' := And.right assum_t;
   sorry
+--   induction jt with
+--   | tyVar y_elem_env =>
+--     sorry
+--     -- cases y_elem_env with
+--     -- | intro y_ty y_elem_env' =>
+--     --   cases y_elem_env' with
+--     --   | Or.inl y_is_x =>
+--     --     rw [←y_is_x]
+--     --     apply js
+--     --   | Or.inr y_elem_env'' =>
+--     --     apply tyVar
+--     --     apply y_elem_env''
+--   | tyAbs jt' =>
+
+--     apply tyAbs
+--     apply jt'
+--   | tyApp jt1 jt2 ihe1 ihe2 =>
+--     apply tyApp
+--     apply ihe1
+--     apply ihe2
 
 theorem preservation :
   Γ ⊢ e : T →
   e —→ e' →
   Γ ⊢ e' : T
 := by
-  intro je eve;
+  intro je;
+  revert e';
   induction je with
   | tyVar =>
     -- Contradictory to ev bacause var cannot be evaluated
+    intros
     contradiction
   | tyAbs =>
     -- Contradictory to ev bacause lam is a value and no rules evaluate it
+    intros
     contradiction
   | tyApp je1 je2 ihe1 ihe2 =>
+    intros e' eve
     cases eve with
     -- eAppAbs : ∀ (t : Ty) (e v : Term), value v → (app (lam t e) v) —→ (subst e 0 v)
     | eAppAbs v_is_value =>
-      sorry
+      apply subst_preservation
+      apply je2
+      apply And.intro
+      cases je1 with
+      | tyAbs jt =>
+        apply jt
+        trivial
     -- eAppLeft : ∀ (e1 e1' e2 : Term), e1 —→ e1' → (app e1 e2) —→ (app e1' e2)
     | eAppLeft eve1 =>
-      sorry
+      apply tyApp
+      apply ihe1
+      apply eve1
+      apply je2
     -- eAppRight : ∀ (v e2 e2' : Term), value v → e2 —→ e2' → (app v e2) —→ (app v e2')
     | eAppRight v_is_value eve2 =>
-      sorry
+      apply tyApp
+      apply je1
+      apply ihe2
+      apply eve2
