lakefile.lean
@@ -1,6 +1,6 @@
 import Lake
 open Lake DSL
-require std from git "https://github.com/leanprover/std4" @ "main"
+-- require std from git "https://github.com/leanprover/std4" @ "main"
 
 package «snlean» where
   -- add package configuration options here
